First commit --- Type Checker implemented. Need to do strong normalization.

dist/Compare_dec.hs
@@ -1,0 +1,107 @@
+module Compare_dec where
+
+import qualified Prelude
+import qualified Datatypes
+import qualified Logic
+import qualified Specif
+
+
+zerop :: Datatypes.Coq_nat -> Prelude.Bool
+zerop n =
+  case n of {
+   Datatypes.O -> Prelude.True;
+   Datatypes.S n0 -> Prelude.False}
+
+lt_eq_lt_dec :: Datatypes.Coq_nat -> Datatypes.Coq_nat -> Prelude.Maybe
+                Prelude.Bool
+lt_eq_lt_dec n =
+  Datatypes.nat_rec (\m ->
+    case m of {
+     Datatypes.O -> Prelude.Just Prelude.False;
+     Datatypes.S m0 -> Prelude.Just Prelude.True}) (\n0 iHn m ->
+    case m of {
+     Datatypes.O -> Prelude.Nothing;
+     Datatypes.S m0 -> iHn m0}) n
+
+gt_eq_gt_dec :: Datatypes.Coq_nat -> Datatypes.Coq_nat -> Prelude.Maybe
+                Prelude.Bool
+gt_eq_gt_dec n m =
+  lt_eq_lt_dec n m
+
+le_lt_dec :: Datatypes.Coq_nat -> Datatypes.Coq_nat -> Prelude.Bool
+le_lt_dec n =
+  Datatypes.nat_rec (\m -> Prelude.True) (\n0 iHn m ->
+    case m of {
+     Datatypes.O -> Prelude.False;
+     Datatypes.S m0 ->
+      Specif.sumbool_rec (\_ -> Prelude.True) (\_ -> Prelude.False) (iHn m0)})
+    n
+
+le_le_S_dec :: Datatypes.Coq_nat -> Datatypes.Coq_nat -> Prelude.Bool
+le_le_S_dec n m =
+  le_lt_dec n m
+
+le_ge_dec :: Datatypes.Coq_nat -> Datatypes.Coq_nat -> Prelude.Bool
+le_ge_dec n m =
+  Specif.sumbool_rec (\_ -> Prelude.True) (\_ -> Prelude.False)
+    (le_lt_dec n m)
+
+le_gt_dec :: Datatypes.Coq_nat -> Datatypes.Coq_nat -> Prelude.Bool
+le_gt_dec n m =
+  le_lt_dec n m
+
+le_lt_eq_dec :: Datatypes.Coq_nat -> Datatypes.Coq_nat -> Prelude.Bool
+le_lt_eq_dec n m =
+  let {s = lt_eq_lt_dec n m} in
+  case s of {
+   Prelude.Just s0 -> s0;
+   Prelude.Nothing -> Logic.coq_False_rec}
+
+le_dec :: Datatypes.Coq_nat -> Datatypes.Coq_nat -> Prelude.Bool
+le_dec n m =
+  le_gt_dec n m
+
+lt_dec :: Datatypes.Coq_nat -> Datatypes.Coq_nat -> Prelude.Bool
+lt_dec n m =
+  le_dec (Datatypes.S n) m
+
+gt_dec :: Datatypes.Coq_nat -> Datatypes.Coq_nat -> Prelude.Bool
+gt_dec n m =
+  lt_dec m n
+
+ge_dec :: Datatypes.Coq_nat -> Datatypes.Coq_nat -> Prelude.Bool
+ge_dec n m =
+  le_dec m n
+
+nat_compare :: Datatypes.Coq_nat -> Datatypes.Coq_nat ->
+               Datatypes.Coq_comparison
+nat_compare n m =
+  case n of {
+   Datatypes.O ->
+    case m of {
+     Datatypes.O -> Datatypes.Eq;
+     Datatypes.S n0 -> Datatypes.Lt};
+   Datatypes.S n' ->
+    case m of {
+     Datatypes.O -> Datatypes.Gt;
+     Datatypes.S m' -> nat_compare n' m'}}
+
+nat_compare_alt :: Datatypes.Coq_nat -> Datatypes.Coq_nat ->
+                   Datatypes.Coq_comparison
+nat_compare_alt n m =
+  case lt_eq_lt_dec n m of {
+   Prelude.Just s ->
+    case s of {
+     Prelude.True -> Datatypes.Lt;
+     Prelude.False -> Datatypes.Eq};
+   Prelude.Nothing -> Datatypes.Gt}
+
+leb :: Datatypes.Coq_nat -> Datatypes.Coq_nat -> Datatypes.Coq_bool
+leb m x =
+  case m of {
+   Datatypes.O -> Datatypes.Coq_true;
+   Datatypes.S m' ->
+    case x of {
+     Datatypes.O -> Datatypes.Coq_false;
+     Datatypes.S n' -> leb m' n'}}
+
