dist/Context.hs
@@ -1,0 +1,43 @@
+module Context where
+
+import qualified Prelude
+import qualified Datatypes
+import qualified Utils
+
+
+type Coq_finite_map a =
+  Datatypes.Coq_list (Datatypes.Coq_prod Utils.Coq_id a)
+
+empty :: Coq_finite_map a1
+empty =
+  Datatypes.Coq_nil
+
+extend :: Utils.Coq_id -> a1 -> (Coq_finite_map a1) -> Datatypes.Coq_list
+          (Datatypes.Coq_prod Utils.Coq_id a1)
+extend x t gamma =
+  case gamma of {
+   Datatypes.Coq_nil -> Datatypes.Coq_cons (Datatypes.Coq_pair x t)
+    Datatypes.Coq_nil;
+   Datatypes.Coq_cons p gam ->
+    case p of {
+     Datatypes.Coq_pair y t' ->
+      case Utils.eq_id_dec x y of {
+       Prelude.True -> Datatypes.Coq_cons (Datatypes.Coq_pair y t) gam;
+       Prelude.False -> Datatypes.Coq_cons (Datatypes.Coq_pair y t')
+        (extend x t gam)}}}
+
+lookup :: Utils.Coq_id -> (Coq_finite_map a1) -> Datatypes.Coq_option a1
+lookup x gamma =
+  case gamma of {
+   Datatypes.Coq_nil -> Datatypes.None;
+   Datatypes.Coq_cons p gam ->
+    case p of {
+     Datatypes.Coq_pair y t' ->
+      case Utils.eq_id_dec x y of {
+       Prelude.True -> Datatypes.Some t';
+       Prelude.False -> lookup x gam}}}
+
+eq_rew_r_dep :: a1 -> a1 -> a2 -> a2
+eq_rew_r_dep x y hC =
+  hC
+
