dist/EqNat.hs
@@ -1,0 +1,28 @@
+module EqNat where
+
+import qualified Prelude
+import qualified Datatypes
+
+
+eq_nat_decide :: Datatypes.Coq_nat -> Datatypes.Coq_nat -> Prelude.Bool
+eq_nat_decide n =
+  Datatypes.nat_rec (\m ->
+    case m of {
+     Datatypes.O -> Prelude.True;
+     Datatypes.S n0 -> Prelude.False}) (\n0 iHn m ->
+    case m of {
+     Datatypes.O -> Prelude.False;
+     Datatypes.S n1 -> iHn n1}) n
+
+beq_nat :: Datatypes.Coq_nat -> Datatypes.Coq_nat -> Datatypes.Coq_bool
+beq_nat n m =
+  case n of {
+   Datatypes.O ->
+    case m of {
+     Datatypes.O -> Datatypes.Coq_true;
+     Datatypes.S n0 -> Datatypes.Coq_false};
+   Datatypes.S n1 ->
+    case m of {
+     Datatypes.O -> Datatypes.Coq_false;
+     Datatypes.S m1 -> beq_nat n1 m1}}
+
