dist/Peano.hs
@@ -1,0 +1,33 @@
+module Peano where
+
+import qualified Prelude
+import qualified Datatypes
+
+
+pred :: Datatypes.Coq_nat -> Datatypes.Coq_nat
+pred n =
+  case n of {
+   Datatypes.O -> n;
+   Datatypes.S u -> u}
+
+plus :: Datatypes.Coq_nat -> Datatypes.Coq_nat -> Datatypes.Coq_nat
+plus n m =
+  case n of {
+   Datatypes.O -> m;
+   Datatypes.S p -> Datatypes.S (plus p m)}
+
+mult :: Datatypes.Coq_nat -> Datatypes.Coq_nat -> Datatypes.Coq_nat
+mult n m =
+  case n of {
+   Datatypes.O -> Datatypes.O;
+   Datatypes.S p -> plus m (mult p m)}
+
+minus :: Datatypes.Coq_nat -> Datatypes.Coq_nat -> Datatypes.Coq_nat
+minus n m =
+  case n of {
+   Datatypes.O -> n;
+   Datatypes.S k ->
+    case m of {
+     Datatypes.O -> n;
+     Datatypes.S l -> minus k l}}
+
