dist/Peano_dec.hs
@@ -1,0 +1,23 @@
+module Peano_dec where
+
+import qualified Prelude
+import qualified Datatypes
+import qualified Specif
+
+
+coq_O_or_S :: Datatypes.Coq_nat -> Prelude.Maybe Datatypes.Coq_nat
+coq_O_or_S n =
+  Datatypes.nat_rec Prelude.Nothing (\n0 iHn -> Prelude.Just n0) n
+
+eq_nat_dec :: Datatypes.Coq_nat -> Datatypes.Coq_nat -> Prelude.Bool
+eq_nat_dec n =
+  Datatypes.nat_rec (\m ->
+    case m of {
+     Datatypes.O -> Prelude.True;
+     Datatypes.S m0 -> Prelude.False}) (\n0 iHn m ->
+    case m of {
+     Datatypes.O -> Prelude.False;
+     Datatypes.S m0 ->
+      Specif.sumbool_rec (\_ -> Prelude.True) (\_ -> Prelude.False) (iHn m0)})
+    n
+
