dist/SfLib.hs
@@ -1,0 +1,72 @@
+module SfLib where
+
+import qualified Prelude
+import qualified Datatypes
+import qualified EqNat
+import qualified Logic
+import qualified Peano_dec
+import qualified Specif
+
+
+ble_nat :: Datatypes.Coq_nat -> Datatypes.Coq_nat -> Datatypes.Coq_bool
+ble_nat n m =
+  case n of {
+   Datatypes.O -> Datatypes.Coq_true;
+   Datatypes.S n' ->
+    case m of {
+     Datatypes.O -> Datatypes.Coq_false;
+     Datatypes.S m' -> ble_nat n' m'}}
+
+type Coq_relation x = ()
+
+next_nat_rect :: Datatypes.Coq_nat -> a1 -> Datatypes.Coq_nat -> a1
+next_nat_rect n f n0 =
+  f
+
+next_nat_rec :: Datatypes.Coq_nat -> a1 -> Datatypes.Coq_nat -> a1
+next_nat_rec n f n0 =
+  next_nat_rect n f n0
+
+empty_relation_rect :: Datatypes.Coq_nat -> Datatypes.Coq_nat -> a1
+empty_relation_rect n n0 =
+  Prelude.error "absurd case"
+
+empty_relation_rec :: Datatypes.Coq_nat -> Datatypes.Coq_nat -> a1
+empty_relation_rec n n0 =
+  empty_relation_rect n n0
+
+type Coq_id =
+  Datatypes.Coq_nat
+  -- singleton inductive, whose constructor was Id
+  
+id_rect :: (Datatypes.Coq_nat -> a1) -> Coq_id -> a1
+id_rect f i =
+  f i
+
+id_rec :: (Datatypes.Coq_nat -> a1) -> Coq_id -> a1
+id_rec =
+  id_rect
+
+beq_id :: Coq_id -> Coq_id -> Datatypes.Coq_bool
+beq_id id1 id2 =
+  EqNat.beq_nat id1 id2
+
+type Coq_partial_map a = Coq_id -> Datatypes.Coq_option a
+
+empty :: Coq_partial_map a1
+empty x =
+  Datatypes.None
+
+extend :: (Coq_partial_map a1) -> Coq_id -> a1 -> Coq_id ->
+          Datatypes.Coq_option a1
+extend gamma x t x' =
+  case beq_id x x' of {
+   Datatypes.Coq_true -> Datatypes.Some t;
+   Datatypes.Coq_false -> gamma x'}
+
+eq_id_dec :: Coq_id -> Coq_id -> Prelude.Bool
+eq_id_dec i i' =
+  id_rec (\n i'0 ->
+    Specif.sumbool_rec (\_ -> Logic.eq_rec_r i'0 Prelude.True n) (\_ ->
+      Prelude.False) (Peano_dec.eq_nat_dec n i'0)) i i'
+
