dist/Specif.hs
@@ -1,0 +1,142 @@
+module Specif where
+
+import qualified Prelude
+import qualified Datatypes
+import qualified Logic
+
+
+__ :: any
+__ = Prelude.error "Logical or arity value used"
+
+type Coq_sig a =
+  a
+  -- singleton inductive, whose constructor was exist
+  
+sig_rect :: (a1 -> () -> a2) -> a1 -> a2
+sig_rect f s =
+  f s __
+
+sig_rec :: (a1 -> () -> a2) -> a1 -> a2
+sig_rec =
+  sig_rect
+
+type Coq_sig2 a =
+  a
+  -- singleton inductive, whose constructor was exist2
+  
+sig2_rect :: (a1 -> () -> () -> a2) -> (Coq_sig2 a1) -> a2
+sig2_rect f s =
+  f s __ __
+
+sig2_rec :: (a1 -> () -> () -> a2) -> (Coq_sig2 a1) -> a2
+sig2_rec =
+  sig2_rect
+
+data Coq_sigT a p =
+   Coq_existT a p
+
+sigT_rect :: (a1 -> a2 -> a3) -> (Coq_sigT a1 a2) -> a3
+sigT_rect f s =
+  case s of {
+   Coq_existT x x0 -> f x x0}
+
+sigT_rec :: (a1 -> a2 -> a3) -> (Coq_sigT a1 a2) -> a3
+sigT_rec =
+  sigT_rect
+
+data Coq_sigT2 a p q =
+   Coq_existT2 a p q
+
+sigT2_rect :: (a1 -> a2 -> a3 -> a4) -> (Coq_sigT2 a1 a2 a3) -> a4
+sigT2_rect f s =
+  case s of {
+   Coq_existT2 x x0 x1 -> f x x0 x1}
+
+sigT2_rec :: (a1 -> a2 -> a3 -> a4) -> (Coq_sigT2 a1 a2 a3) -> a4
+sigT2_rec =
+  sigT2_rect
+
+proj1_sig :: a1 -> a1
+proj1_sig e =
+  e
+
+projT1 :: (Coq_sigT a1 a2) -> a1
+projT1 x =
+  case x of {
+   Coq_existT a p -> a}
+
+projT2 :: (Coq_sigT a1 a2) -> a2
+projT2 x =
+  case x of {
+   Coq_existT x0 h -> h}
+
+sig_of_sigT :: (Coq_sigT a1 ()) -> a1
+sig_of_sigT x =
+  case x of {
+   Coq_existT x0 _ -> x0}
+
+sigT_of_sig :: a1 -> Coq_sigT a1 ()
+sigT_of_sig x =
+  Coq_existT x __
+
+sumbool_rect :: (() -> a1) -> (() -> a1) -> Prelude.Bool -> a1
+sumbool_rect f f0 s =
+  case s of {
+   Prelude.True -> f __;
+   Prelude.False -> f0 __}
+
+sumbool_rec :: (() -> a1) -> (() -> a1) -> Prelude.Bool -> a1
+sumbool_rec =
+  sumbool_rect
+
+sumor_rect :: (a1 -> a2) -> (() -> a2) -> (Prelude.Maybe a1) -> a2
+sumor_rect f f0 s =
+  case s of {
+   Prelude.Just x -> f x;
+   Prelude.Nothing -> f0 __}
+
+sumor_rec :: (a1 -> a2) -> (() -> a2) -> (Prelude.Maybe a1) -> a2
+sumor_rec =
+  sumor_rect
+
+coq_Choice :: (a1 -> a2) -> (a1 -> a2)
+coq_Choice h z =
+  proj1_sig (h z)
+
+coq_Choice2 :: (a1 -> Coq_sigT a2 a3) -> Coq_sigT (a1 -> a2) (a1 -> a3)
+coq_Choice2 h =
+  Coq_existT (\z -> projT1 (h z)) (\z ->
+    let {s = h z} in
+    case s of {
+     Coq_existT x r -> r})
+
+bool_choice :: (a1 -> Prelude.Bool) -> (a1 -> Datatypes.Coq_bool)
+bool_choice h z =
+  case h z of {
+   Prelude.True -> Datatypes.Coq_true;
+   Prelude.False -> Datatypes.Coq_false}
+
+dependent_choice :: (a1 -> a1) -> a1 -> (Datatypes.Coq_nat -> a1)
+dependent_choice h x0 n =
+  case n of {
+   Datatypes.O -> x0;
+   Datatypes.S n' -> proj1_sig (h (dependent_choice h x0 n'))}
+
+type Exc a = Datatypes.Coq_option a
+
+value :: a1 -> Datatypes.Coq_option a1
+value x =
+  Datatypes.Some x
+
+error :: Datatypes.Coq_option a1
+error =
+  Datatypes.None
+
+except :: a1
+except =
+  Logic.coq_False_rec
+
+absurd_set :: a1
+absurd_set =
+  Logic.coq_False_rec
+
