dist/Subtype.hs
@@ -1,0 +1,24 @@
+module Subtype where
+
+import qualified Prelude
+import qualified Ty
+
+
+sectyof :: Ty.Coq_ty -> Ty.Coq_secty
+sectyof t =
+  case t of {
+   Ty.Coq_ty_bool s -> s;
+   Ty.Coq_arrow t0 t1 s -> s}
+
+lub_secty :: Ty.Coq_secty -> Ty.Coq_secty -> Ty.Coq_secty
+lub_secty x y =
+  case x of {
+   Ty.Trust -> y;
+   Ty.Untrust -> Ty.Untrust}
+
+update_secty :: Ty.Coq_ty -> Ty.Coq_secty -> Ty.Coq_ty
+update_secty t s =
+  case t of {
+   Ty.Coq_ty_bool s' -> Ty.Coq_ty_bool (lub_secty s s');
+   Ty.Coq_arrow l r s' -> Ty.Coq_arrow l r (lub_secty s s')}
+
