dist/Syntax.hs
@@ -1,0 +1,41 @@
+module Syntax where
+
+import qualified Prelude
+import qualified Ty
+import qualified Utils
+
+
+data Coq_term =
+   Coq_tm_false
+ | Coq_tm_true
+ | Coq_tm_var Utils.Coq_id
+ | Coq_tm_app Coq_term Coq_term
+ | Coq_tm_abs Utils.Coq_id Ty.Coq_ty Coq_term
+ | Coq_tm_trust Coq_term
+ | Coq_tm_distrust Coq_term
+ | Coq_tm_check Coq_term
+
+term_rect :: a1 -> a1 -> (Utils.Coq_id -> a1) -> (Coq_term -> a1 -> Coq_term
+             -> a1 -> a1) -> (Utils.Coq_id -> Ty.Coq_ty -> Coq_term -> a1 ->
+             a1) -> (Coq_term -> a1 -> a1) -> (Coq_term -> a1 -> a1) ->
+             (Coq_term -> a1 -> a1) -> Coq_term -> a1
+term_rect f f0 f1 f2 f3 f4 f5 f6 t =
+  case t of {
+   Coq_tm_false -> f;
+   Coq_tm_true -> f0;
+   Coq_tm_var i -> f1 i;
+   Coq_tm_app t0 t1 ->
+    f2 t0 (term_rect f f0 f1 f2 f3 f4 f5 f6 t0) t1
+      (term_rect f f0 f1 f2 f3 f4 f5 f6 t1);
+   Coq_tm_abs i t0 t1 -> f3 i t0 t1 (term_rect f f0 f1 f2 f3 f4 f5 f6 t1);
+   Coq_tm_trust t0 -> f4 t0 (term_rect f f0 f1 f2 f3 f4 f5 f6 t0);
+   Coq_tm_distrust t0 -> f5 t0 (term_rect f f0 f1 f2 f3 f4 f5 f6 t0);
+   Coq_tm_check t0 -> f6 t0 (term_rect f f0 f1 f2 f3 f4 f5 f6 t0)}
+
+term_rec :: a1 -> a1 -> (Utils.Coq_id -> a1) -> (Coq_term -> a1 -> Coq_term
+            -> a1 -> a1) -> (Utils.Coq_id -> Ty.Coq_ty -> Coq_term -> a1 ->
+            a1) -> (Coq_term -> a1 -> a1) -> (Coq_term -> a1 -> a1) ->
+            (Coq_term -> a1 -> a1) -> Coq_term -> a1
+term_rec =
+  term_rect
+
