dist/Ty.hs
@@ -1,0 +1,75 @@
+module Ty where
+
+import qualified Prelude
+import qualified Datatypes
+import qualified Logic
+import qualified Peano
+import qualified Specif
+
+
+data Coq_secty =
+   Trust
+ | Untrust
+
+secty_rect :: a1 -> a1 -> Coq_secty -> a1
+secty_rect f f0 s =
+  case s of {
+   Trust -> f;
+   Untrust -> f0}
+
+secty_rec :: a1 -> a1 -> Coq_secty -> a1
+secty_rec =
+  secty_rect
+
+secty_eq_dec :: Coq_secty -> Coq_secty -> Prelude.Bool
+secty_eq_dec s s' =
+  secty_rec (\s'0 ->
+    case s'0 of {
+     Trust -> Prelude.True;
+     Untrust -> Prelude.False}) (\s'0 ->
+    case s'0 of {
+     Trust -> Prelude.False;
+     Untrust -> Prelude.True}) s s'
+
+data Coq_ty =
+   Coq_ty_bool Coq_secty
+ | Coq_arrow Coq_ty Coq_ty Coq_secty
+
+ty_rect :: (Coq_secty -> a1) -> (Coq_ty -> a1 -> Coq_ty -> a1 -> Coq_secty ->
+           a1) -> Coq_ty -> a1
+ty_rect f f0 t =
+  case t of {
+   Coq_ty_bool s -> f s;
+   Coq_arrow t0 t1 s -> f0 t0 (ty_rect f f0 t0) t1 (ty_rect f f0 t1) s}
+
+ty_rec :: (Coq_secty -> a1) -> (Coq_ty -> a1 -> Coq_ty -> a1 -> Coq_secty ->
+          a1) -> Coq_ty -> a1
+ty_rec =
+  ty_rect
+
+ty_eq_dec :: Coq_ty -> Coq_ty -> Prelude.Bool
+ty_eq_dec t t' =
+  ty_rec (\s0 t'0 ->
+    case t'0 of {
+     Coq_ty_bool s1 ->
+      Specif.sumbool_rec (\_ -> Logic.eq_rec_r s1 Prelude.True s0) (\_ ->
+        Prelude.False) (secty_eq_dec s0 s1);
+     Coq_arrow t0 t1 s1 -> Prelude.False}) (\t0 h t1 h0 s0 t'0 ->
+    case t'0 of {
+     Coq_ty_bool s1 -> Prelude.False;
+     Coq_arrow t2 t3 s1 ->
+      Specif.sumbool_rec (\_ ->
+        Logic.eq_rec_r t2
+          (Specif.sumbool_rec (\_ ->
+            Logic.eq_rec_r t3
+              (Specif.sumbool_rec (\_ -> Logic.eq_rec_r s1 Prelude.True s0)
+                (\_ -> Prelude.False) (secty_eq_dec s0 s1)) t1) (\_ ->
+            Prelude.False) (h0 t3)) t0) (\_ -> Prelude.False) (h t2)}) t t'
+
+ty_size :: Coq_ty -> Datatypes.Coq_nat
+ty_size t =
+  case t of {
+   Coq_ty_bool s -> Datatypes.O;
+   Coq_arrow l r s ->
+    Peano.plus (Peano.plus (Datatypes.S Datatypes.O) (ty_size l)) (ty_size r)}
+
