dist/TypeChecker.hs
@@ -1,0 +1,133 @@
+module TypeChecker where
+
+import qualified Prelude
+import qualified Context
+import qualified Datatypes
+import qualified Peano
+import qualified Specif
+import qualified Subtype
+import qualified Syntax
+import qualified Ty
+import qualified Utils
+
+
+sec_ordering_dec :: Ty.Coq_secty -> Ty.Coq_secty -> Prelude.Bool
+sec_ordering_dec s s' =
+  case s of {
+   Ty.Trust -> Prelude.True;
+   Ty.Untrust ->
+    case s' of {
+     Ty.Trust -> Prelude.False;
+     Ty.Untrust -> Prelude.True}}
+
+typair_size :: Ty.Coq_ty -> Ty.Coq_ty -> Datatypes.Coq_nat
+typair_size t t' =
+  Peano.plus (Ty.ty_size t) (Ty.ty_size t')
+
+eq_rew_dep :: a1 -> a2 -> a1 -> a2
+eq_rew_dep x f y =
+  f
+
+subtype_dec_func :: (Specif.Coq_sigT Ty.Coq_ty Ty.Coq_ty) -> Prelude.Bool
+subtype_dec_func x =
+  let {t = Specif.projT1 x} in
+  let {t' = Specif.projT2 x} in
+  let {
+   subtype_dec0 = \t0 t'0 ->
+    let {y = Specif.Coq_existT t0 t'0} in
+    subtype_dec_func (Specif.proj1_sig y)}
+  in
+  case t of {
+   Ty.Coq_ty_bool s ->
+    case t' of {
+     Ty.Coq_ty_bool s' -> sec_ordering_dec s s';
+     Ty.Coq_arrow t0 t1 s0 -> Prelude.False};
+   Ty.Coq_arrow l r s ->
+    case t' of {
+     Ty.Coq_ty_bool s0 -> Prelude.False;
+     Ty.Coq_arrow l' r' s' ->
+      let {filtered_var = subtype_dec0 l' l} in
+      let {filtered_var0 = subtype_dec0 r r'} in
+      let {filtered_var1 = sec_ordering_dec s s'} in
+      case filtered_var of {
+       Prelude.True ->
+        case filtered_var0 of {
+         Prelude.True -> filtered_var1;
+         Prelude.False -> Prelude.False};
+       Prelude.False -> Prelude.False}}}
+
+subtype_dec :: Ty.Coq_ty -> Ty.Coq_ty -> Prelude.Bool
+subtype_dec t t' =
+  subtype_dec_func (Specif.Coq_existT t t')
+
+trustworth :: Ty.Coq_ty -> Prelude.Bool
+trustworth t =
+  Ty.secty_rec (\s ->
+    case s of {
+     Ty.Trust -> Prelude.True;
+     Ty.Untrust -> Prelude.False}) (\s ->
+    case s of {
+     Ty.Trust -> Prelude.False;
+     Ty.Untrust -> Prelude.True}) (Subtype.sectyof t) Ty.Trust
+
+var_dec :: Utils.Coq_id -> (Context.Coq_finite_map Ty.Coq_ty) ->
+           Prelude.Maybe Ty.Coq_ty
+var_dec i ctx =
+  let {o = Context.lookup i ctx} in
+  case o of {
+   Datatypes.Some t -> Prelude.Just t;
+   Datatypes.None -> Prelude.Nothing}
+
+arrow_split :: Ty.Coq_ty -> Prelude.Maybe
+               (Datatypes.Coq_prod Ty.Coq_ty Ty.Coq_ty)
+arrow_split t =
+  case t of {
+   Ty.Coq_ty_bool s -> Prelude.Nothing;
+   Ty.Coq_arrow t1 t2 s -> Prelude.Just (Datatypes.Coq_pair t1 t2)}
+
+is_a_bool_ty :: Ty.Coq_ty -> Prelude.Bool
+is_a_bool_ty t =
+  case t of {
+   Ty.Coq_ty_bool s -> Prelude.True;
+   Ty.Coq_arrow t1 t2 s -> Prelude.False}
+
+typecheck_dec :: Syntax.Coq_term -> (Context.Coq_finite_map Ty.Coq_ty) ->
+                 Prelude.Maybe Ty.Coq_ty
+typecheck_dec e ctx =
+  case e of {
+   Syntax.Coq_tm_var i -> var_dec i ctx;
+   Syntax.Coq_tm_app l r ->
+    case typecheck_dec l ctx of {
+     Prelude.Just s ->
+      case typecheck_dec r ctx of {
+       Prelude.Just s0 ->
+        case arrow_split s of {
+         Prelude.Just s1 ->
+          case subtype_dec s0 (Datatypes.fst s1) of {
+           Prelude.True -> Prelude.Just
+            (Subtype.update_secty (Datatypes.snd s1) (Subtype.sectyof s));
+           Prelude.False -> Prelude.Nothing};
+         Prelude.Nothing -> Prelude.Nothing};
+       Prelude.Nothing -> Prelude.Nothing};
+     Prelude.Nothing -> Prelude.Nothing};
+   Syntax.Coq_tm_abs i ty e0 ->
+    case typecheck_dec e0 (Context.extend i ty ctx) of {
+     Prelude.Just s -> Prelude.Just (Ty.Coq_arrow ty s Ty.Trust);
+     Prelude.Nothing -> Prelude.Nothing};
+   Syntax.Coq_tm_trust t ->
+    case typecheck_dec t ctx of {
+     Prelude.Just s -> Prelude.Just (Subtype.update_secty s Ty.Trust);
+     Prelude.Nothing -> Prelude.Nothing};
+   Syntax.Coq_tm_distrust t ->
+    case typecheck_dec t ctx of {
+     Prelude.Just s -> Prelude.Just (Subtype.update_secty s Ty.Untrust);
+     Prelude.Nothing -> Prelude.Nothing};
+   Syntax.Coq_tm_check t ->
+    case typecheck_dec t ctx of {
+     Prelude.Just s ->
+      case trustworth s of {
+       Prelude.True -> Prelude.Just s;
+       Prelude.False -> Prelude.Nothing};
+     Prelude.Nothing -> Prelude.Nothing};
+   _ -> Prelude.Just (Ty.Coq_ty_bool Ty.Trust)}
+
