dist/Utils.hs
@@ -1,0 +1,51 @@
+module Utils where
+
+import qualified Prelude
+import qualified Compare_dec
+import qualified Datatypes
+import qualified EqNat
+import qualified Logic
+import qualified Peano_dec
+import qualified Specif
+
+
+type Coq_id =
+  Datatypes.Coq_nat
+  -- singleton inductive, whose constructor was Id
+  
+id_rect :: (Datatypes.Coq_nat -> a1) -> Coq_id -> a1
+id_rect f i =
+  f i
+
+id_rec :: (Datatypes.Coq_nat -> a1) -> Coq_id -> a1
+id_rec =
+  id_rect
+
+beq_id :: Coq_id -> Coq_id -> Datatypes.Coq_bool
+beq_id i i' =
+  EqNat.beq_nat i i'
+
+eq_id_dec :: Coq_id -> Coq_id -> Prelude.Bool
+eq_id_dec i i' =
+  id_rec (\n i'0 ->
+    Specif.sumbool_rec (\_ -> Logic.eq_rec_r i'0 Prelude.True n) (\_ ->
+      Prelude.False) (Peano_dec.eq_nat_dec n i'0)) i i'
+
+lt_eq_lt_id_dec :: Coq_id -> Coq_id -> Prelude.Maybe Prelude.Bool
+lt_eq_lt_id_dec i1 i2 =
+  case Compare_dec.lt_eq_lt_dec i1 i2 of {
+   Prelude.Just s ->
+    case s of {
+     Prelude.True -> Prelude.Just Prelude.True;
+     Prelude.False -> Logic.eq_rec_r i2 (Prelude.Just Prelude.False) i1};
+   Prelude.Nothing ->
+    case Compare_dec.lt_dec i2 i1 of {
+     Prelude.True -> Prelude.Nothing;
+     Prelude.False -> Logic.coq_False_rec}}
+
+type Coq_relation x = ()
+
+ex_falso_quodlibet :: a1
+ex_falso_quodlibet =
+  Prelude.error "absurd case"
+
