dist/Wf0.hs
@@ -1,0 +1,52 @@
+module Wf0 where
+
+import qualified Prelude
+import qualified Logic
+import qualified Specif
+import qualified Wf
+
+
+__ :: any
+__ = Prelude.error "Logical or arity value used"
+
+coq_Fix_F_sub :: (a1 -> (a1 -> a2) -> a2) -> a1 -> a2
+coq_Fix_F_sub f_sub x =
+  f_sub x (\y -> coq_Fix_F_sub f_sub (Specif.proj1_sig y))
+
+coq_Fix_sub :: (a1 -> (a1 -> a2) -> a2) -> a1 -> a2
+coq_Fix_sub f_sub x =
+  f_sub x (\y -> coq_Fix_sub f_sub (Specif.proj1_sig y))
+
+coq_Fix_F_sub_rect :: (a1 -> (a1 -> a2) -> a2) -> (a1 -> (a1 -> () -> () ->
+                      a3) -> () -> a3) -> a1 -> a3
+coq_Fix_F_sub_rect f inv x =
+  Wf.well_founded_induction_type (\x0 x1 _ ->
+    Logic.eq_rect_r
+      (f x0 (\y ->
+        let {
+         fix_F_sub x2 =
+           f x2 (\y0 -> fix_F_sub (Specif.proj1_sig y0))}
+        in fix_F_sub (Specif.proj1_sig y))) (inv x0 x1 __)
+      (let {
+        fix_F_sub x2 =
+          f x2 (\y -> fix_F_sub (Specif.proj1_sig y))}
+       in fix_F_sub x0)) x __
+
+coq_Fix_sub_rect :: (a1 -> (a1 -> a2) -> a2) -> (a1 -> (a1 -> () -> a3) -> ()
+                    -> a3) -> a1 -> a3
+coq_Fix_sub_rect f inv x =
+  coq_Fix_F_sub_rect f (\x0 x1 _ ->
+    let {x2 = \y -> x1 y __ __} in
+    let {q = inv x0 (\y _ -> x2 y) __} in
+    Logic.eq_rect
+      (f x0 (\y ->
+        let {
+         fix_F_sub x3 =
+           f x3 (\y0 -> fix_F_sub (Specif.proj1_sig y0))}
+        in fix_F_sub (Specif.proj1_sig y))) q
+      (f x0 (\y ->
+        let {
+         fix_F_sub x3 =
+           f x3 (\y0 -> fix_F_sub (Specif.proj1_sig y0))}
+        in fix_F_sub (Specif.proj1_sig y)))) x
+
