Syntax.v
@@ -1,12 +1,11 @@
 
-Require Import SfLib Ty.
+Require Import Utils Ty.
 
 (** simple sytax definition for the calculus**)
 
 Inductive term : Type :=
   | tm_false : term
   | tm_true : term
-  | tm_if : term -> term -> term -> term
   | tm_var : id -> term
   | tm_app : term -> term -> term
   | tm_abs : id -> ty -> term -> term
@@ -15,6 +14,6 @@ Inductive term : Type :=
   | tm_check : term -> term.
 
 Tactic Notation "term_cases" tactic(first) ident(c) :=
-  first ; [Case_aux c "tm_false" | Case_aux c "tm_true" | Case_aux c "tm_if" | 
+  first ; [Case_aux c "tm_false" | Case_aux c "tm_true" | 
            Case_aux c "tm_var" | Case_aux c "tm_app"  | Case_aux c "tm_abs" |
            Case_aux c "tm_trust" | Case_aux c "tm_distrust" | Case_aux c "tm_check"].
