Ty.v
@@ -1,8 +1,8 @@
 (** Definition of types **)
 
-Require Import SfLib MinMax.
+Require Import Utils MinMax.
 
-Inductive secty : Type := Trust : secty | Untrust : secty | DontCare : secty.
+Inductive secty : Type := Trust : secty | Untrust : secty.
 
 Definition secty_eq_dec : forall (s s' : secty), {s = s'} + {s <> s'}.
   decide equality.
@@ -14,14 +14,11 @@ Inductive ty : Type :=
 
 Definition ty_eq_dec : forall (t t' : ty), {t = t'} + {t <> t'}.
   pose secty_eq_dec.
-  pose eq_id_dec.
   decide equality.
 Defined.
 
 Tactic Notation "ty_cases" tactic(first) ident(c) :=
   first ; [Case_aux c "base" | Case_aux c "arrow"].
-
-Definition context := partial_map ty.
 
 (** definition of a type size,
     this is used to ensure termination
