TypeSystem.v
@@ -1,26 +1,20 @@
+Require Import Utils Context Syntax Ty Subtype Semantics.
 
-Require Import SfLib Syntax Ty Subtype Semantics.
+(** Definition of the type system -- non syntax directed version**)
 
-(** Definition of the type system **)
-
-Inductive has_type : context -> term -> ty -> Prop :=
+Inductive has_type : finite_map ty -> term -> ty -> Prop :=
   | T_True : forall ctx, has_type ctx tm_true (ty_bool Trust)
   | T_False : forall ctx, has_type ctx tm_false (ty_bool Trust)
   | T_Var : forall ctx v ty, 
-        ctx v = Some ty -> has_type ctx (tm_var v) ty
+               lookup v ctx = Some ty -> has_type ctx (tm_var v) ty
   | T_Abs : forall ctx x t2 T1 T2, 
-        has_type (extend ctx x T1) t2 T2 ->
+        has_type (extend x T1 ctx) t2 T2 ->
         has_type ctx (tm_abs x T1 t2) (arrow T1 T2 Trust)
-  | T_App : forall ctx t1 t2 T11 T11' T12 s, 
+  | T_App : forall ctx t1 t2 T11 T12 s, 
         has_type ctx t1 (arrow T11 T12 s) -> 
-        has_type ctx t2 T11' ->
-        subtype T11' T11     ->
+        has_type ctx t2 T11 ->
+        (** subtype T11' T11     -> **)
         has_type ctx (tm_app t1 t2) (update_secty T12 s)
-  | T_If : forall ctx t1 t2 t3 T s,
-        has_type ctx t1 (ty_bool s) ->
-        has_type ctx t2 T     ->
-        has_type ctx t3 T     -> 
-        has_type ctx (tm_if t1 t2 t3) T
   | T_Trust : forall ctx t T,
         has_type ctx t T ->
         has_type ctx (tm_trust t) (update_secty T Trust)
@@ -38,9 +32,8 @@ Inductive has_type : context -> term -> ty -> Prop :=
                                      
 Tactic Notation "has_type_cases" tactic(first) ident(c) :=
   first ; [Case_aux c "T_True"  | Case_aux c "T_False"   | Case_aux c "T_Var"   |
-           Case_aux c "T_Abs"   | Case_aux c "T_App"     | Case_aux c "T_If"    |
-           Case_aux c "T_Trust" | Case_aux c "T_Untrust" | Case_aux c "T_Check" |
-           Case_aux c "T_Sub"].
+           Case_aux c "T_Abs"   | Case_aux c "T_App"     | Case_aux c "T_Trust" | 
+           Case_aux c "T_Untrust" | Case_aux c "T_Check" | Case_aux c "T_Sub"].
 
 Hint Constructors has_type.
 
@@ -51,7 +44,7 @@ Lemma sub_inversion_base :
 Proof with eauto.
   intros T s Hsub.
   remember (ty_bool s) as V.
-  subtype_cases (induction Hsub) Case ; try (inv HeqV) ; try (eexists ; eauto ; fail).
+  subtype_cases (induction Hsub) Case ; try (inv HeqV) ; try (eexists ; split ; eauto).
 Qed. 
 
 Lemma sub_inversion_arrow : 
@@ -96,8 +89,8 @@ Lemma canonical_forms_bool :
 Proof with eauto.
   intros ctx t s Hty Hv ; remember (ty_bool s) as V.
   generalize dependent s.
-  has_type_cases (induction Hty) Case ; try intros ; try solve by inversion 2 ...
-  subst.
+  has_type_cases (induction Hty) Case ; try intros ; try solve by inversion 2.
+  left ... right ... subst.
   apply sub_inversion_base in H.
   destruct H as [s' [Heq Hs]].
   eapply IHHty ...
@@ -113,7 +106,7 @@ Proof with eauto.
   remember (@empty ty) as Gamma.
   generalize dependent HeqGamma.
   has_type_cases (induction Hty) Case ; 
-  intros Heq ; subst ; try (solve by inversion) ...
+  intros Heq ; subst ; try (solve by inversion) ; try (left ; eauto ; fail) ...  
   Case "T_App".
     right.
     destruct IHHty1 ; subst ...
@@ -124,31 +117,19 @@ Proof with eauto.
           as [x [S1 [s2 Heq]]] ... subst.
         exists (subst x t2 s2) ...
       SSCase "t2 can step".
-         destruct H1 as [t2' Ht'] ; exists (tm_app t1 t2') ...
-    SCase "t1 can step".
-      destruct H0 as [t1' Ht1'].
-      exists (tm_app t1' t2) ...
-  Case "T_If".
-    destruct IHHty1 ...
-    SCase "t1 is a value".
-      assert (Hb : t1 = tm_true \/ t1 = tm_false) by
-        (eapply canonical_forms_bool ; eauto).
-      inv Hb ...
+         destruct H0 as [t2' Ht'] ; exists (tm_app t1 t2') ...
     SCase "t1 can step".
       destruct H as [t1' Ht1'].
-      right ; exists (tm_if t1' t2 t3) ...
+      exists (tm_app t1' t2) ...
   Case "T_Trust".
     destruct IHHty ...
-    destruct H as [t' Ht'].
-    right. exists (tm_trust t') ...
+    destruct H as [t' Ht'] ; right ; exists (tm_trust t') ...
   Case "T_Untrust".
     destruct IHHty ...
-    destruct H as [t' Ht'].
-    right. exists (tm_distrust t') ...
+    destruct H as [t' Ht'] ; right ; exists (tm_distrust t') ...
   Case "T_Check".
     destruct IHHty ...
-    destruct H0 as [t' Ht'].
-    right. exists (tm_check t') ...
+    destruct H0 as [t' Ht'] ; right ; exists (tm_check t') ...
 Qed.
 
 (** inversion lemmas for the typing relation *)
@@ -156,7 +137,7 @@ Qed.
 Lemma typing_inversion_abs : 
   forall ctx x S1 s2 T, has_type ctx (tm_abs x S1 s2) T ->
     exists S2,  subtype (arrow S1 S2 Trust) T /\
-      has_type (extend ctx x S1) s2 S2.
+      has_type (extend x S1 ctx) s2 S2.
 Proof with eauto.
   intros ctx x S1 s2 T H.
   remember (tm_abs x S1 s2) as t.
@@ -164,12 +145,12 @@ Proof with eauto.
   Case "T_Abs".
     exists T2 ; split ...   
   Case "T_Sub".
-    destruct IHhas_type as [S2 [H1 H2]] ...
+    destruct IHhas_type as [S2 [H1 H2]] ; repeat (eexists ; split ; eauto).
 Qed.
 
 Lemma typing_inversion_var : 
   forall ctx x T, has_type ctx (tm_var x) T ->
-    exists S, ctx x = Some S /\ subtype S T.
+    exists S, lookup x ctx = Some S /\ subtype S T.
 Proof with eauto.
   intros ctx x T Hty.
   remember (tm_var x) as V.
@@ -203,8 +184,8 @@ Qed.
 
 Lemma typing_inversion_app :
   forall ctx t1 t2 T2, has_type ctx (tm_app t1 t2) T2 ->
-    exists T1, exists T11, exists s, 
-      has_type ctx t1 (arrow T1 T2 s) /\ has_type ctx t2 T11 /\ subtype T11 T1 /\ sectyof T2 = sectyof (update_secty T2 s).
+    exists T1, exists s, 
+      has_type ctx t1 (arrow T1 T2 s) /\ has_type ctx t2 T1 /\ sectyof T2 = sectyof (update_secty T2 s).
 Proof with eauto.
   intros ctx t1 t2 T2 Hty.
   remember (tm_app t1 t2) as t.
@@ -214,7 +195,7 @@ Proof with eauto.
     rewrite <- update_secty_ident ...
   Case "T_Sub".
     destruct IHHty ...
-    destruct H0 as [T11 [s [H1 [H2 [H3 H4]]]]].
+    destruct H0 as [s1 [H1 [H2 H3]]].
     repeat eexists ... eapply secty_update_eq ...
 Qed.
 
@@ -257,22 +238,10 @@ Proof with eauto.
     destruct IHHty as [T1 [H1 [H2 H3]]] ...
 Qed.
 
-Lemma typing_inversion_if :
-  forall ctx t1 t2 t3 T, has_type ctx (tm_if t1 t2 t3) T ->
-    exists s, has_type ctx t1 (ty_bool s) /\ has_type ctx t2 T /\ has_type ctx t3 T.
-Proof with eauto.
-  intros ctx t1 t2 t3 T Hty.
-  remember (tm_if t1 t2 t3) as V.
-  has_type_cases (induction Hty) Case ; inv HeqV ; try solve by inversion ...
-  Case "T_Sub".
-    destruct IHHty as [s [H1 [H2 H3]]] ...
-    eexists ; repeat split ...
-Qed.
-
 Lemma abs_arrow : 
   forall x S1 s2 T1 T2 s,
     has_type empty (tm_abs x S1 s2) (arrow T1 T2 s) ->
-    subtype T1 S1 /\ has_type (extend empty x S1) s2 T2.
+    subtype T1 S1 /\ has_type (extend x S1 empty) s2 T2.
 Proof with eauto.
   intros x S1 s2 T1 T2 s Hty.
   apply typing_inversion_abs in Hty.
@@ -292,12 +261,6 @@ Inductive appears_free_in : id -> term -> Prop :=
                                appears_free_in i (tm_app t1 t2)
   | afi_abs : forall i x T t, i <> x -> appears_free_in i t ->
                               appears_free_in i (tm_abs x T t)
-  | afi_if1 : forall i t1 t2 t3, appears_free_in i t1 ->
-                                 appears_free_in i (tm_if t1 t2 t3)
-  | afi_if2 : forall i t1 t2 t3, appears_free_in i t2 ->
-                                 appears_free_in i (tm_if t1 t2 t3)
-  | afi_if3 : forall i t1 t2 t3, appears_free_in i t3 ->
-                                 appears_free_in i (tm_if t1 t2 t3)
   | afi_trust : forall i t, appears_free_in i t ->
                             appears_free_in i (tm_trust t)
   | afi_distrust : forall i t, appears_free_in i t ->
@@ -306,41 +269,59 @@ Inductive appears_free_in : id -> term -> Prop :=
                             appears_free_in i (tm_check t).
 
 Hint Constructors appears_free_in.
+
+Definition closed (t : term) := ~ (exists v, appears_free_in v t).
   
 Lemma context_invariance :
   forall ctx ctx' t S, has_type ctx t S ->
-    (forall x, appears_free_in x t -> ctx x = ctx' x) ->
+    (forall x, appears_free_in x t -> lookup x ctx = lookup x ctx') ->
     has_type ctx' t S.
 Proof with eauto.
-  intros. generalize dependent ctx'.
+  intros ctx ctx' t S H. generalize dependent ctx'.
   has_type_cases (induction H) Case ; intros ctx' Heqv ; try solve by inversion ...
   Case "T_Var".
     apply T_Var. rewrite <- Heqv...
   Case "T_Abs".
     apply T_Abs ...
-    apply IHhas_type. intros x0 Hafi ; unfold extend.
+    apply IHhas_type. intros x0 Hafi.
     remember (beq_id x x0) as e ; destruct e ...
     symmetry in Heqe.
-    apply beq_id_false_not_eq in Heqe ...
+    apply beq_id_true_eq in Heqe ...
+    subst.
+    rewrite extend_lookup ; rewrite extend_lookup ; auto.
+    symmetry in Heqe. apply beq_id_false_not_eq in Heqe.
+    assert (x0 <> x). intro Hc ; unfold not in Heqe ; symmetry in Hc ; contradiction.
+    apply extend_lookup_neq with (g := ctx) (t := T1) in H0.
+    rewrite H0.
+    assert (x0 <> x). intro Hc ; unfold not in Heqe ; symmetry in Hc ; contradiction.
+    apply extend_lookup_neq with (g := ctx') (t := T1) in H1.
+    rewrite H1 ; auto.
   Case "T_App".
     eapply T_App ...
-  Case "T_If".
-    eapply T_If ...
 Qed.
 
 Lemma free_in_context :
   forall i ctx t T,
     appears_free_in i t ->
     has_type ctx t T ->
-    exists T', ctx i = Some T'.
+    exists T', lookup i ctx = Some T'.
 Proof with eauto.
   intros i ctx t T Hafi Hty.
   has_type_cases (induction Hty) Case ; inv Hafi ...
   Case "T_Abs".
-    destruct (IHHty H4) as [T Ht]. exists T. unfold extend in Ht.
-    apply not_eq_beq_id_false in H2. rewrite beq_id_sym in H2.
+    destruct (IHHty H4) as [T Ht]. exists T.
+    apply extend_lookup_neq with (t := T1) (g := ctx) in H2.
     rewrite H2 in Ht ...
 Qed.
+
+
+Corollary typable_empty__closed : forall t T,
+    has_type empty t T ->
+    closed t.
+Proof.
+  intros t T H. unfold closed. intros H1 ; destruct H1 as [x H2].
+  destruct (free_in_context _ _ _ _ H2 H) as [T' C].
+  inversion C. Qed.
 
 (** substitution lemma **)
 
@@ -348,7 +329,7 @@ Hint Resolve typing_inversion_false typing_inversion_true.
 
 Lemma substitution_preserves_typing : 
   forall Gamma x U v t S,
-    has_type (extend Gamma x U) t S ->
+    has_type (extend x U Gamma) t S ->
     has_type empty v U ->
     has_type Gamma (subst x v t) S.
 Proof with eauto.
@@ -361,33 +342,31 @@ Proof with eauto.
   Case "tm_true".
      apply typing_inversion_true in Htypt.
      eapply T_Sub ...
-  Case "tm_if".
-     assert (exists s, has_type (extend Gamma x U) t1 (ty_bool s) /\ 
-                       has_type (extend Gamma x U) t2 S /\ 
-                       has_type (extend Gamma x U) t3 S)
-       by apply (typing_inversion_if _ _ _ _ _ Htypt)...
-     destruct H as [s [H1 [H2 H3]]]...
   Case "tm_var".
      destruct (typing_inversion_var _ _ _ Htypt) as [T [H1 H2]].
-     unfold extend in H1.
      remember (beq_id x i) as e ; destruct e.
      SCase "x = i".
-       apply beq_id_eq in Heqe ; inv H1.
+       symmetry in Heqe.
+       apply beq_id_true_eq in Heqe. subst.
+       rewrite extend_lookup in H1. inv H1.
+       apply T_Sub with (T := T)...
        apply context_invariance with empty ...
-       intros x contra.
-       destruct (free_in_context _ empty _ T contra) ...      
-       inv H.
+       intros x contra.       
+       destruct (free_in_context _ empty _ T contra) ; try solve by inversion...      
      SCase "x <> i".
        symmetry in Heqe.
        apply beq_id_false_not_eq in Heqe.
-       apply T_Sub with T ...
+       apply context_invariance with (extend x U Gamma)...
+       intros x1 contra. inv contra.
+       apply extend_lookup_neq. 
+       intro Hc ; symmetry in Hc ; unfold not in Heqe ; contradiction.
    Case "tm_app".
-     destruct (typing_inversion_app _ _ _ _ Htypt) as [T1 [T11 [s [H1 [H2 [H3 H4]]]]]].  
+     destruct (typing_inversion_app _ _ _ _ Htypt) as [T [s [H1 [H2 H3]]]].
      apply IHt1 in H1.
      apply IHt2 in H2.
      eapply T_Sub.  
      eapply T_App...
-     destruct S ; simpl in * ; rewrite <- H4 ...
+     destruct S ; simpl in * ; rewrite <- H3 ...
    Case "tm_abs".
      rename i into y. rename t into T1.
      destruct (typing_inversion_abs _ _ _ _ _ Htypt) as [T2 [H1 H2]].
@@ -395,14 +374,18 @@ Proof with eauto.
      remember (beq_id x y) as e ; destruct e.
      SCase "x = y".
        eapply context_invariance ...       
-       apply beq_id_eq in Heqe ; subst.
-       intros x0 Hafi ; unfold extend.
+       symmetry in Heqe. apply beq_id_true_eq in Heqe ; subst.
+       intros x0 Hafi.
        destruct (beq_id y x0) ...
+       rewrite extend_override ...
+       rewrite extend_override...
      SCase "x <> y".
        apply IHt. eapply context_invariance ...
-       intros z Hafi. unfold extend.
+       intros z Hafi. symmetry in Heqe. apply beq_id_false_not_eq in Heqe.
        remember (beq_id y z) as e1 ; destruct e1...
-       apply beq_id_eq in Heqe1. subst. rewrite <- Heqe ...
+       eapply extend_swap_neq in Heqe ...
+       symmetry in Heqe1. apply beq_id_false_not_eq in Heqe1. 
+       eapply extend_swap_neq in Heqe ...
    Case "tm_trust".
      destruct (typing_inversion_trust _ _ _ Htypt) as [T [H1 H2]].
      apply T_Sub with (update_secty T Trust) ...
@@ -428,4 +411,76 @@ Proof with eauto.
    SCase "ST_AppAbs".
      destruct (abs_arrow _ _ _ _ _ _ HT1) as [HA1 HA2].
      apply substitution_preserves_typing with T ...
+Qed.
+
+(** syntax directed system **)
+
+Inductive has_type_alg : finite_map ty -> term -> ty -> Prop :=
+  | TA_True : forall ctx, has_type_alg ctx tm_true (ty_bool Trust)
+  | TA_False : forall ctx, has_type_alg ctx tm_false (ty_bool Trust)
+  | TA_Var : forall ctx v ty, 
+        lookup v ctx = Some ty -> has_type_alg ctx (tm_var v) ty
+  | TA_Abs : forall ctx x t2 T1 T2, 
+        has_type_alg (extend x T1 ctx) t2 T2 ->
+        has_type_alg ctx (tm_abs x T1 t2) (arrow T1 T2 Trust)
+  | TA_App : forall ctx t1 t2 T11 T11' T12 s, 
+        has_type_alg ctx t1 (arrow T11 T12 s) -> 
+        has_type_alg ctx t2 T11' ->
+        subtype T11' T11     ->
+        has_type_alg ctx (tm_app t1 t2) (update_secty T12 s)
+  | TA_Trust : forall ctx t T,
+        has_type_alg ctx t T ->
+        has_type_alg ctx (tm_trust t) (update_secty T Trust)
+  | TA_Untrust : forall ctx t T,
+        has_type_alg ctx t T ->
+        has_type_alg ctx (tm_distrust t) (update_secty T Untrust)
+  | TA_Check : forall ctx t T,
+        has_type_alg ctx t T ->
+        sectyof T = Trust ->
+        has_type_alg ctx (tm_check t) T. 
+
+Hint Constructors has_type_alg.
+
+Theorem has_type_alg_soundness : 
+  forall ctx t ty, has_type_alg ctx t ty -> has_type ctx t ty.
+Proof.
+  intros ctx t ty H ; induction H ; eauto.
+Qed.
+
+Theorem has_type_alg_completeness : 
+  forall ctx t ty, has_type ctx t ty -> exists ty', has_type_alg ctx t ty' /\ subtype ty' ty.
+Proof with eauto.
+  Hint Resolve update_secty_mono.
+  intros ctx t ty H ; has_type_cases (induction H) Case ; try (eexists ; split ; eauto ; fail).
+  Case "T_Abs".
+    destruct IHhas_type as [T [HT HS]].
+    apply TA_Abs in HT ; eexists ; split ...
+  Case "T_App".
+    destruct IHhas_type1 as [T1 [HT1 HS1]].
+    destruct IHhas_type2 as [T2 [HT2 HS2]].
+    apply sub_inversion_arrow in HS1. destruct HS1 as [s1 [T1' [T2' [HE [HS1' [HS2' HS3]]]]]] ; subst.
+    eexists ; split ...
+  Case "T_Trust".
+    destruct IHhas_type as [T' [HT' HS]].
+    eexists ; split ...     
+  Case "T_Untrust".
+    destruct IHhas_type as [T' [HT' HS]].
+    eexists ; split ...
+  Case "T_Check".
+    destruct IHhas_type as [T' [HT' HS]].
+    eexists ; split ; try constructor ... 
+  Case "T_Sub".
+    destruct IHhas_type as [T1 [HT1 HS]].
+    eexists ; split ...
+Qed.
+
+Theorem has_type_alg_unique : 
+  forall ctx t T, has_type_alg ctx t T -> forall T', has_type_alg ctx t T' -> T = T'.
+Proof with eauto.
+  intros ctx t T HT ; induction HT ; intros T' HT' ; inv HT' ; auto.
+  rewrite H in H2 ; inv H2 ; auto.
+  apply IHHT in H4 ; subst ; auto.
+  apply IHHT1 in H2 ; inv H2 ; auto.
+  apply IHHT in H1 ; subst ; auto.
+  apply IHHT in H1 ; subst ; auto.
 Qed.
