Simulation.v
@@ -1,0 +1,96 @@
+Require Import Context Stlc TypeSystem Syntax Ty Subtype List Utils Semantics.
+
+(** Erasure **)
+
+Fixpoint erase_ty (t : ty) : stlc_ty :=
+  match t with
+    | ty_bool _ => stlc_bool
+    | arrow l r _ => stlc_arrow (erase_ty l) (erase_ty r)
+  end.
+
+Fixpoint erase_term (t : term) : stlc_term :=
+  match t  with
+    | tm_false => stlc_false
+    | tm_true => stlc_true
+    | tm_var i => stlc_var i
+    | tm_app l r => stlc_app (erase_term l) (erase_term r)
+    | tm_abs i T t => stlc_abs i (erase_ty T) (erase_term t)
+    | tm_trust t => erase_term t
+    | tm_distrust t => erase_term t
+    | tm_check t => erase_term t
+  end.
+
+Definition erase_context (ctx : finite_map ty) : stlc_context :=
+  map (fun p => match p with 
+                  | (i,t) => (i, erase_ty t)
+                end) ctx.
+
+(** lemma 12 **)
+
+Lemma subtype_erase : forall T T', subtype T T' -> erase_ty T = erase_ty T'.
+Proof.
+  intros T T' H ; induction H ; simpl ; f_equal ; auto.
+Qed.
+
+(** Theorem 13 **)
+
+Lemma lookup_erase : forall i (t : ty) g, lookup i g = Some t -> lookup i (erase_context g) = Some (erase_ty t).
+Proof.
+  intros i t g H.
+  induction g ; try solve by inversion.
+  destruct a. simpl. remember (eq_id_dec i i0) as e ; destruct e ; subst ;auto.
+  simpl in H. rewrite <- Heqe in H. inv H. auto.
+  apply IHg. simpl in H. rewrite <- Heqe in H. auto.
+Qed.
+
+Lemma extend_erase : forall i (t : ty) g, erase_context (extend i t g) = extend i (erase_ty t) (erase_context g).
+Proof.
+  intros i t g ; induction g.
+  simpl ; auto.
+  destruct a ; simpl.
+  remember (eq_id_dec i i0) as e ; destruct e ; subst ; auto.
+  simpl. f_equal ; auto.
+Qed.
+
+Lemma update_secty_erase : forall t s, erase_ty (update_secty t s) = erase_ty t.
+Proof.
+  intros t s ; induction t ; simpl ; auto.
+Qed.
+
+Lemma subst_erase : forall x v t, erase_term (subst x v t) = Stlc.subst x (erase_term v) (erase_term t).
+Proof.
+  intros x v t ; induction t ; simpl ;  
+    try (match goal with
+           [ |- context[if beq_id ?X ?Y then _ else _]] => remember (beq_id X Y) as e ; destruct e
+         end) ; auto.
+   rewrite <- IHt1. rewrite <- IHt2. auto.
+   rewrite <- IHt ; auto.
+Qed.
+
+Lemma value_erase : forall t, value t -> stlc_value (erase_term t).
+Proof.
+  intros t H ; inv H ; simpl ; auto.
+Qed. 
+
+Hint Resolve lookup_erase subtype_erase value_erase.
+
+Theorem erase_typing : forall ctx e T, has_type ctx e T -> stlc_has_type (erase_context ctx) (erase_term e) (erase_ty T).
+Proof with eauto.
+  intros ctx e T HT.
+  induction HT ; simpl ; try econstructor ...
+  rewrite <- extend_erase ... 
+  rewrite -> update_secty_erase ...
+  rewrite -> update_secty_erase ...
+  rewrite -> update_secty_erase ...
+  apply subtype_erase in H.
+  rewrite <- H ...
+Qed.
+
+(** simulation **)
+
+Theorem simulation : forall ctx t T, has_type ctx t T -> exists v, (erase_term t) ==>s* v -> exists g, t ==>* g /\ (erase_term g) = v.
+Proof.
+  intros ctx t T HT.
+  induction t ; try (eexists ; intros ; eexists ; split ; eauto ; try econstructor; fail).
+Qed.  
+
