Stlc.v
@@ -1,0 +1,94 @@
+(** Standard definitions of a simple typed lambda calculus
+    with booleans **)
+
+Require Import Utils Context.
+
+(** syntax definition **)
+
+Inductive stlc_ty : Type :=
+  | stlc_bool : stlc_ty
+  | stlc_arrow : stlc_ty -> stlc_ty -> stlc_ty.
+
+Inductive stlc_term : Type :=
+  | stlc_true : stlc_term
+  | stlc_false : stlc_term
+  | stlc_var : id -> stlc_term
+  | stlc_app : stlc_term -> stlc_term -> stlc_term
+  | stlc_abs : id -> stlc_ty -> stlc_term -> stlc_term.
+
+(** Semantics **)
+
+Fixpoint subst (x : id) (t : stlc_term) (t' : stlc_term) {struct t'} : stlc_term :=
+  match t' with
+    | stlc_var i      => if beq_id x i then t else t'
+    | stlc_app l r    => stlc_app (subst x t l) (subst x t r)
+    | stlc_abs i T t1 => stlc_abs i T (if beq_id x i then t1 else (subst x t t1))
+    | stlc_true       => stlc_true
+    | stlc_false      => stlc_false
+  end.
+
+Inductive stlc_bvalue : stlc_term -> Prop :=
+  | sv_true : stlc_bvalue stlc_true 
+  | sv_false : stlc_bvalue stlc_false.
+
+Inductive stlc_absvalue : stlc_term -> Prop :=
+  | sv_abs : forall x T t12, stlc_absvalue (stlc_abs x T t12).
+
+Definition stlc_value (t : stlc_term) : Prop := stlc_bvalue t \/ stlc_absvalue t.
+
+Hint Constructors stlc_bvalue stlc_absvalue.
+Hint Unfold stlc_value.
+
+Reserved Notation "t '==>s' t'" (at level 40). 
+
+Inductive stlc_step : stlc_term -> stlc_term -> Prop :=
+  | se_appabs : forall x T t12 v2, stlc_value v2 -> (stlc_app (stlc_abs x T t12) v2) ==>s subst x v2 t12
+  | se_app1   : forall t1 t1' t2, t1 ==>s t1' -> stlc_app t1 t2 ==>s stlc_app t1' t2
+  | se_app2   : forall v1 t2 t2', stlc_value v1 -> t2 ==>s t2' -> stlc_app v1 t2 ==>s stlc_app v1 t2'
+  where "t '==>s' t'" := (stlc_step t t').
+
+Hint Constructors stlc_step.
+
+Definition stlc_multi_step := refl_step_closure stlc_step.
+
+Notation "t '==>s*' t'" := (stlc_multi_step t t') (at level 40).
+
+Remark value_dont_step : forall t, stlc_value t -> ~ exists t', t ==>s t'.
+Proof.
+  intros t H Hc ;
+  inv H ; inv H0 ; destruct Hc ; solve by inversion.
+Qed.
+
+Ltac s := f_equal ; eauto ;
+  match goal with
+    | [H : stlc_value ?X, H1 : ?X ==>s _ |- _] =>
+        apply value_dont_step in H ; elim H ; eexists 
+  end.
+
+Lemma step_deterministic : forall t t', t ==>s t' -> forall t'', t ==>s t'' -> t' = t''.
+Proof.
+   induction 1 ; intros t'' H2 ; inv H2 ;
+   try solve by inversion ; repeat s.
+Qed.
+
+(** typing **)
+
+Definition stlc_context := finite_map stlc_ty.
+
+Inductive stlc_has_type : stlc_context -> stlc_term -> stlc_ty -> Prop :=
+  | ST_Var : forall Gamma x T,
+      lookup x Gamma = Some T ->
+      stlc_has_type Gamma (stlc_var x) T
+  | ST_Abs : forall Gamma x T11 T12 t12,
+      stlc_has_type (extend x T11 Gamma) t12 T12 -> 
+      stlc_has_type Gamma (stlc_abs x T11 t12) (stlc_arrow T11 T12)
+  | ST_App : forall T11 T12 Gamma t1 t2,
+      stlc_has_type Gamma t1 (stlc_arrow T11 T12) -> 
+      stlc_has_type Gamma t2 T11 -> 
+      stlc_has_type Gamma (stlc_app t1 t2) T12
+  | ST_True : forall Gamma,
+       stlc_has_type Gamma stlc_true stlc_bool
+  | ST_False : forall Gamma,
+       stlc_has_type Gamma stlc_false stlc_bool.
+
+Hint Constructors stlc_has_type.
