TypeChecker.v
@@ -1,8 +1,8 @@
 (** Implementation of a typechecker for
     the trust calculus **)
 
-Require Import SfLib Tactics Syntax TypeSystem Subtype.
-Require Import Wf Wellfounded.Lexicographic_Product.
+Require Import Utils Context Tactics Syntax TypeSystem Subtype.
+Require Import Wf Wellfounded.Lexicographic_Product Coq.Program.Tactics Omega.
 Require Import Relation_Operators Transitive_Closure Recdef Program MinMax.
 Require Import Ty.
 
@@ -14,11 +14,10 @@ Definition sec_ordering_dec : forall (s s' : secty), {sec_ordering s s'} + {~ se
      fun (s s' : secty) => 
          match s, s' with
            | Trust, Untrust => _
-           | Untrust, DontCare => _
-           | Trust, DontCare => _
-           | DontCare ,DontCare => _
-           | _ , _ => _
-         end
+           | Untrust, Trust => _
+           | Trust, Trust => _
+           | Untrust, Untrust => _
+        end
     ) ; auto ; right ; intro H ; try solve by inversion.
 Defined.
 
@@ -33,9 +32,15 @@ Ltac my_tac :=
          | [H : arrow _ _ _ = ty_bool _ |- _] => inv H
          | [H : ty_bool _ = arrow _ _ _ |- _] => inv H
          | [|- _ /\ _] => split
+         | [H : ex _ |- _] => destruct H
+         | [H : Some _ = Some _ |- _] => inv H
+         | [H : None = Some _ |- _] => congruence
+         | [H : ?X -> False |- False] => apply H
        end) ; eauto.
 
-Obligation Tactic := try my_tac ; (simpl ; omega).
+Ltac s := try (repeat my_tac) ; (simpl ; try omega).
+
+Obligation Tactic := s.
 
 Program Fixpoint subtype_dec (t t' : ty) {measure (typair_size t t')} : {subtype t t'} + {~ subtype t t'} :=
   match t,t' with
@@ -54,4 +59,94 @@ Program Fixpoint subtype_dec (t t' : ty) {measure (typair_size t t')} : {subtype
          end
     | _, _ => right _
   end.
+
+Definition trustworth (t : ty) : {sectyof t = Trust} + {~ sectyof t = Trust}.
+  decide equality.
+Defined.
+
+(** Defining the typechecker itself **)  
+
+
+Ltac start := 
+     repeat
+       (match goal with
+         | [H : forall _, _ |- _] => intro ; start
+         | [H : ~ _ |- _] => intro ; clear H
+         | [H : ex _ |- _] => destruct H
+         | [|- has_type_alg _ _ _] => econstructor (solve [eauto])
+         | [H : (ty * ty)%type |- _] => destruct H
+       end ; try subst ; simpl) ; eauto.
+
+Definition var_dec : forall i (ctx : finite_map ty), {t | lookup i ctx = Some t} + {~ exists t, lookup i ctx = Some t}.
+  intros i ctx.
+  destruct (lookup i ctx) ; [left ; eexists | right ; intro] ; eauto.
+  destruct H. inv H.
+Defined.
+
+Definition arrow_split (t : ty) : {(t1,t2) : ty * ty | exists s, t = arrow t1 t2 s} + 
+                                  {~ (exists t1, exists t2, exists s, t = arrow t1 t2 s)}.
+  destruct t.
+  right. intro H. destruct H as [t1 [t2 [s' H]]] ; inv H.
+  left . exists (t1,t2). exists s. auto.
+Defined. 
+
+Definition is_a_bool_ty : forall (t : ty), {exists s, subtype t (ty_bool s)} + 
+                                           {~ exists s, subtype t (ty_bool s)}.
+   intros t ; destruct t.
+   left. destruct s ; [exists Trust | exists Untrust] ; auto.
+   right. intro H. destruct H as [s1 H1] ; inv H1.
+Defined.
+
+Definition typecheck_dec : forall(e : term) (ctx : finite_map ty), 
+  {t | has_type_alg ctx e t} + {forall t, ~ has_type_alg ctx e t}.
+  refine (fix F (e : term) (ctx : finite_map ty) {struct e}: 
+     {t | has_type_alg ctx e t} + {forall t, ~ has_type_alg ctx e t} :=
+     match e return {t | has_type_alg ctx e t} + {forall t, ~ has_type_alg ctx e t} with
+       | tm_true => [|| (ty_bool Trust) ||]
+       | tm_false => [|| (ty_bool Trust) ||]
+       | tm_var i => 
+           match var_dec i ctx with
+             | inleft (exist t _) => [|| t ||]
+             | inright _ => !!
+           end
+       | tm_abs i ty e =>
+            ty' <-- F e (extend i ty ctx) ;
+            [|| arrow ty ty' Trust ||]
+       | tm_app l r => 
+            tf <-- F l ctx ;
+            ta <-- F r ctx ;
+            p  <-- arrow_split tf ;
+            subtype_dec ta (fst p) ;;;
+            [|| update_secty (snd p) (sectyof tf) ||]
+       | tm_trust t  => 
+            ty <-- F t ctx ;
+            [|| update_secty ty Trust ||]
+       | tm_distrust t => 
+            ty <-- F t ctx ;
+            [|| update_secty ty Untrust ||]
+       | tm_check t => 
+            ty <-- F t ctx ;
+            trustworth ty ;;;
+            [|| ty ||]
+     end) ; start. 
+     elim n ; inv H ; eexists ; eauto.
+     simpl in *.
+     destruct s1 as [[t2 t3] [s' He]] ; inv He.
+     inv H.
+     apply (has_type_alg_unique _ _ _ H2) in h ; inv h.
+     apply (has_type_alg_unique _ _ _ h0) in H4 ; inv H4.
+     contradiction.
+     inv H ; elim n. 
+     apply (has_type_alg_unique _ _ _ H2) in h ; inv h.
+     exists T11 ; exists T12 ; exists s1 ; auto.
+     inv H ; apply n in H4 ; auto.
+     inv H ; apply n in H2 ; auto.
+     inv H ; apply n in H5 ; auto.
+     inv H ; apply n in H2 ; auto.
+     inv H ; apply n in H2 ; auto.
+     inv H.
+     apply (has_type_alg_unique _ _ _ h) in H1 ; subst.
+     contradiction.
+     inv H. apply n in H1 ; auto.
+ Defined.
 
