Utils.v
@@ -1,0 +1,197 @@
+(** Utils.v 
+    Some utilities that are used in several places.
+**)
+
+Require Export Bool.
+Require Export List.
+Require Export Arith_base.
+Require Export Arith.EqNat.
+
+(** case tactic **)
+
+Require String. Open Scope string_scope.
+
+Ltac move_to_top x :=
+  match reverse goal with
+  | H : _ |- _ => try move x after H
+  end.
+
+Tactic Notation "assert_eq" ident(x) constr(v) :=
+  let H := fresh in
+  assert (x = v) as H by reflexivity;
+  clear H.
+
+Tactic Notation "Case_aux" ident(x) constr(name) :=
+  first [
+    set (x := name); move_to_top x
+  | assert_eq x name; move_to_top x
+  | fail 1 "because we are working on a different case" ].
+
+Tactic Notation "Case" constr(name) := Case_aux Case name.
+Tactic Notation "SCase" constr(name) := Case_aux SCase name.
+Tactic Notation "SSCase" constr(name) := Case_aux SSCase name.
+Tactic Notation "SSSCase" constr(name) := Case_aux SSSCase name.
+Tactic Notation "SSSSCase" constr(name) := Case_aux SSSSCase name.
+Tactic Notation "SSSSSCase" constr(name) := Case_aux SSSSSCase name.
+Tactic Notation "SSSSSSCase" constr(name) := Case_aux SSSSSSCase name.
+Tactic Notation "SSSSSSSCase" constr(name) := Case_aux SSSSSSSCase name.
+
+(** inv and solve by inversion tactic **)
+
+Ltac inv H := inversion H ; clear H ; subst.
+
+
+Tactic Notation "solve_by_inversion_step" tactic(t) :=
+  (match goal with
+    | H : _ |-  _ => solve [ inversion H; subst; t ]
+    end) || fail "because the goal is not solvable by inversion.".
+
+Tactic Notation "solve" "by" "inversion" "1" :=
+  solve_by_inversion_step idtac.
+Tactic Notation "solve" "by" "inversion" "2" :=
+  solve_by_inversion_step (solve by inversion 1).
+Tactic Notation "solve" "by" "inversion" "3" :=
+  solve_by_inversion_step (solve by inversion 2).
+Tactic Notation "solve" "by" "inversion" :=
+  solve by inversion 1.
+
+(** notations for easy working with subset types **)
+
+Notation "!" := (False_rec _ _).
+Notation "[ e ]" := (exist _ e _).
+
+Notation "!!" := (inright _ _).
+Notation "[|| x ||]" := (inleft _  (exist _ x _) ).
+
+Notation "x <-- e1 ; e2" := (match e1 with
+                               | inright _ => !!
+                               | inleft (exist x _) => e2
+                             end)
+(right associativity, at level 60).
+
+Notation "e1 ;;; e2" := (if e1 then e2 else !!)
+  (right associativity, at level 60).
+
+(** identifiers **)
+
+Inductive id : Type :=
+  | Id : nat -> id.
+
+Definition lt_id (i i' : id) : Prop :=
+  match i, i' with
+    | Id n, Id n' => lt n n'
+  end.
+
+Definition beq_id (i i' : id) : bool :=
+  match i, i' with
+    | Id n, Id n' => beq_nat n n'
+  end.
+
+Lemma beq_id_false_not_eq : forall i i', beq_id i i' = false -> i <> i'.
+Proof.
+  intros i i'.
+  destruct i ; destruct i'.
+  intros H1 H2. inv H2.
+  simpl in H1. apply beq_nat_false in H1 ; elim H1 ; auto.
+Qed.
+
+Lemma beq_id_true_eq : forall i i', beq_id i i' = true -> i = i'.
+Proof.
+  intros i i' H. destruct i ; destruct i' ; f_equal ; simpl in H.
+  apply beq_nat_true ; auto.
+Qed.
+
+Definition eq_id_dec : forall (i i' : id), {i = i'} + {i <> i'}.
+   pose eq_nat_dec.
+   decide equality.
+Defined.
+
+Lemma eq_id_refl : forall (i : id), i = i.
+Proof.
+  auto.
+Qed.
+
+Lemma eq_id_sym : forall (i1 i2 : id), i1 = i2 -> i2 = i1.
+Proof.
+  intros ; symmetry ; auto.
+Qed.
+
+Lemma eq_id_trans : forall (i1 i2 i3 : id), i1 = i2 -> i2 = i3 -> i1 = i3.
+Proof.
+  intros i1 i2 i3 H1 H2. rewrite -> H1. auto.
+Qed.
+
+Lemma lt_id_trans : forall (i1 i2 i3 : id), lt_id i1 i2 -> lt_id i2 i3 -> lt_id i1 i3.
+Proof.
+  intros i1 i2 i3 H1 H2.
+  destruct i1 ; destruct i2 ; destruct i3 ; simpl in *.
+  eapply lt_trans ; eauto.
+Qed.
+
+Lemma lt_id_not_eq_id : forall (i1 i2 : id), lt_id i1 i2 -> i1 <> i2.
+Proof.
+  intros i1 i2 H. destruct i1 ; destruct i2 ; intro contra.
+  rewrite -> contra in H. simpl in H.
+  apply lt_irrefl in H ; auto.
+Qed.
+
+Definition lt_eq_lt_id_dec (i1 i2 : id) : {lt_id i1 i2} + {i1 = i2} + {lt_id i2 i1}.
+   refine (match i1,i2 with 
+             Id n1, Id n2 => match lt_eq_lt_dec n1 n2 with
+                               | inleft _ => _
+                               | inright _ => match lt_dec n2 n1 with
+                                                | left _ => _
+                                                | right _ => _
+                                              end
+                             end
+           end).
+  destruct s. left ; left ; auto.
+  subst ; left ; right ; auto.
+  right ; auto.
+  contradiction.
+Defined. 
+
+(** definitions of reflexive-transitive closure of a relation **)
+
+Definition relation (X: Type) := X -> X -> Prop.
+
+Inductive refl_step_closure {X:Type} (R: relation X) : relation X :=
+  | rsc_refl : forall (x : X), refl_step_closure R x x
+  | rsc_step : forall (x y z : X),
+                    R x y ->
+                    refl_step_closure R y z ->
+                    refl_step_closure R x z.
+
+Hint Constructors refl_step_closure.
+
+Tactic Notation "rsc_cases" tactic(first) ident(c) :=
+  first;
+  [ Case_aux c "rsc_refl" | Case_aux c "rsc_step" ].
+
+Theorem rsc_R : forall (X:Type) (R:relation X) (x y : X),
+       R x y -> refl_step_closure R x y.
+Proof.
+  intros X R x y r.
+  apply rsc_step with y. apply r. apply rsc_refl.   Qed.
+
+Theorem rsc_trans :
+  forall (X:Type) (R: relation X) (x y z : X),
+      refl_step_closure R x y  ->
+      refl_step_closure R y z ->
+      refl_step_closure R x z.
+Proof.
+  intros X R x y z H1.
+  induction H1. trivial.
+  intros H2.
+  apply IHrefl_step_closure in H2.
+  eapply rsc_step ; eassumption ; eauto.
+Qed.
+
+Theorem ex_falso_quodlibet : forall (P:Type),
+  False -> P.
+Proof.
+  intros P contra.
+  inversion contra. Qed.
+
+
+
