Extraction.v~
@@ -1,0 +1,11 @@
+Require Import TypeChecker.
+
+Extraction Language Haskell.
+
+Cd "dist".
+
+Extract Inductive sumbool => "Prelude.Bool" ["Prelude.True" "Prelude.False"].
+Extract Inductive sumor   => "Prelude.Maybe" ["Prelude.Just" "Prelude.Nothing"].
+
+
+Recursive Extraction Library TypeChecker.
